refactoring

tarjan_num.v
@@ -11,60 +11,7 @@ Unset Printing Implicit Defensive.
 Section tarjan.
 
 Variable (V : finType) (successors : V -> seq V).
-Notation edge := (grel successors).
-Notation gconnect := (connect edge).
 Notation infty := #|V|.+1.
-
-(*************************************************)
-(* Connected components of the graph, abstractly *)
-(*************************************************)
-
-Notation gsymconnect := [rel x y | gconnect x y && gconnect y x].
-
-Lemma gsymconnect_equiv : equivalence_rel gsymconnect.
-Proof.
-split; first by rewrite /gsymconnect /= connect0.
-move=> /andP [xy yx]; rewrite /gsymconnect /=.
-by apply/idP/idP => /andP [/(connect_trans _)-> // /connect_trans->].
-Qed.
-
-Definition gsccs := equivalence_partition gsymconnect setT.
-
-Lemma gsccs_partition : partition gsccs setT.
-Proof. by apply: equivalence_partitionP => ?*; apply: gsymconnect_equiv. Qed.
-
-Definition cover_gsccs := cover_partition gsccs_partition.
-
-Lemma trivIset_gsccs : trivIset gsccs.
-Proof. by case/and3P: gsccs_partition. Qed.
-Hint Resolve trivIset_gsccs.
-
-Notation scc_of := (pblock gsccs).
-
-Lemma mem_scc x y : x \in scc_of y = gsymconnect y x.
-Proof.
-by rewrite pblock_equivalence_partition // => ?*; apply: gsymconnect_equiv.
-Qed.
-
-Definition def_scc scc x := @def_pblock _ _ scc x trivIset_gsccs.
-
-Definition is_subscc (A : {set V}) :=
-  A != set0 /\ {in A &, forall x y, gconnect x y}.
-
-Lemma is_subscc_in_scc (A : {set V}) :
-  is_subscc A -> exists2 scc, scc \in gsccs & A \subset scc.
-Proof.
-move=> []; have [->|[x xA]] := set_0Vmem A; first by rewrite eqxx.
-move=> AN0 A_sub; exists (scc_of x); first by rewrite pblock_mem ?cover_gsccs.
-by apply/subsetP => y yA; rewrite mem_scc /= !A_sub //.
-Qed.
-
-Lemma is_subscc1 x (A : {set V}) : x \in A ->
-  (forall y, y \in A -> gconnect x y /\ gconnect y x) -> is_subscc A.
-Proof.
-move=> xA AP; split; first by apply: contraTneq xA => ->; rewrite inE.
-by move=> y z /AP [xy yx] /AP [xz zx]; rewrite (connect_trans yx).
-Qed.
 
 (**********************************************************)
 (*               Tarjan 72 algorithm,                     *)
@@ -74,20 +21,20 @@ Qed.
 Definition split_after (T :eqType) (x : T) (s : seq T) :=
   let i := index x s in (rcons (take i s) x, drop i.+1 s).
 
-Record env := Env {blacks : {set V}; stack : seq V; sccs : {set {set V}};
+Record env := Env {blacks : {set V}; stack : seq V; esccs : {set {set V}};
                    sn : nat; num: {ffun V -> nat}}.
 
 Definition set_infty (s : pred V) f :=
   [ffun x => if s x then infty else f x].
 
 Definition add_stack x e :=
-  Env (blacks e) (x :: stack e) (sccs e) (sn e).+1
+  Env (blacks e) (x :: stack e) (esccs e) (sn e).+1
       (finfun [eta num e with x |-> sn e]).
 Definition add_blacks x e :=
-  Env (x |: blacks e) (stack e) (sccs e) (sn e) (num e).
+  Env (x |: blacks e) (stack e) (esccs e) (sn e) (num e).
 Definition add_sccs x e :=
    let (s2, s3) := split_after x (stack e) in
-   Env (x |: blacks e) s3 ([set y in s2] |: sccs e)
+   Env (x |: blacks e) s3 ([set y in s2] |: esccs e)
        (sn e) (set_infty (mem s2) (num e)).
 
 Definition dfs1 (dfs : {set V} -> env -> nat * env) (x : V) e :=
@@ -106,7 +53,18 @@ Fixpoint tarjan_rec n : {set V} -> env -> nat * env :=
 
 Let N := #|V| * #|V|.+1 + #|V|.
 Definition e0 := (Env set0 [::] set0 1 [ffun _ => 0]).
-Definition tarjan := sccs (tarjan_rec N setT e0).2.
+Definition tarjan := esccs (tarjan_rec N setT e0).2.
+
+(*****************)
+(* Abbreviations *)
+(*****************)
+
+Notation edge := (grel successors).
+Notation gconnect := (connect edge).
+Notation gsymconnect := (symconnect edge).
+Notation gsccs := (sccs edge).
+Notation gscc_of := (pblock gsccs).
+Notation gconnected := (connected edge).
 
 (**************************************************************)
 (* Well formed environements and operations on environements. *)
@@ -207,7 +165,7 @@ Proof. by []. Qed.
 
 Lemma sccs_add_sccs e x :
   let s := take (index x (stack e)) (stack e) in
-  sccs (add_sccs x e) = [set y in rcons s x] |: sccs e.
+  esccs (add_sccs x e) = [set y in rcons s x] |: esccs e.
 Proof. by []. Qed.
 
 Lemma stack_add_sccs e x :
@@ -220,8 +178,8 @@ Proof. by []. Qed.
 (*******************)
 
 Record wf_color e := WfEnv {
-   wf_stack : stack e =i grays e :|: (blacks e :\: cover (sccs e));
-   wf_sccs  : cover (sccs e) \subset blacks e;
+   wf_stack : stack e =i grays e :|: (blacks e :\: cover (esccs e));
+   wf_sccs  : cover (esccs e) \subset blacks e;
    wf_uniq  : uniq (stack e);
 }.
 Hint Resolve wf_sccs.
@@ -229,7 +187,7 @@ Hint Resolve wf_uniq.
 
 Inductive color4_spec x e : bool -> bool -> bool -> bool -> bool -> Type :=
 | Color4Gray of x \in grays e : color4_spec x e false true false true false
-| Color4Sccs of x \in cover (sccs e) :
+| Color4Sccs of x \in cover (esccs e) :
                        color4_spec x e true false true false false
 | Color4White of x \in whites e : color4_spec x e false false false false true
 | Color4BlackStack of x \in blacks e & x \in stack e :
@@ -237,7 +195,7 @@ Inductive color4_spec x e : bool -> bool -> bool -> bool -> bool -> Type :=
 
 Lemma color4P x e : wf_color e ->
                    color4_spec x e (x \in blacks e) (x \in stack e)
-                              (x \in cover (sccs e))
+                              (x \in cover (esccs e))
                               (x \in grays e) (x \in whites e).
 Proof.
 move=> [/(_ x) s_def /subsetP /(_ x) /implyP].
@@ -250,7 +208,7 @@ by constructor; rewrite whitesE graysE !inE x_black x_stack.
 Qed.
 
 Lemma stack_sccsF x e : wf_color e -> x \in stack e ->
-  x \in cover (sccs e) = false.
+  x \in cover (esccs e) = false.
 Proof. by case/color4P. Qed.
 
 Lemma grays_blacksF x e : wf_color e -> x \in grays e ->
@@ -258,14 +216,14 @@ Lemma grays_blacksF x e : wf_color e -> x \in grays e ->
 Proof. by case/color4P. Qed.
 
 Lemma grays_sccsF x e : wf_color e -> x \in grays e ->
-   x \in cover (sccs e) = false.
+   x \in cover (esccs e) = false.
 Proof. by case/color4P. Qed.
 
 Lemma sccs_stackF x e : wf_color e ->
-  x \in cover (sccs e) -> x \in stack e = false.
+  x \in cover (esccs e) -> x \in stack e = false.
 Proof. by case/color4P. Qed.
 
-Lemma sccs_blacks x e : wf_color e -> x \in cover (sccs e) -> x \in blacks e.
+Lemma sccs_blacks x e : wf_color e -> x \in cover (esccs e) -> x \in blacks e.
 Proof. by case/color4P. Qed.
 
 Lemma add_stack_cwf x e : x \in whites e -> wf_color e -> wf_color (add_stack x e).
@@ -314,11 +272,11 @@ Inductive stack_spec x e : bool -> bool -> bool -> bool -> bool -> Type :=
 | StackWhite of x \in whites e : stack_spec x e true false false false false
 | StackStack of x \in stack e :
                        stack_spec x e false true false (x \in grays e) (x \in blacks e)
-| StackSccs  of x \in cover (sccs e) :
+| StackSccs  of x \in cover (esccs e) :
                         stack_spec x e false false true false true.
 
 Lemma stackP x e : wf_color e ->
-  stack_spec x e (x \in whites e) (x \in stack e) (x \in cover (sccs e))
+  stack_spec x e (x \in whites e) (x \in stack e) (x \in cover (esccs e))
                               (x \in grays e) (x \in blacks e).
 Proof.
 move=> e_cwf; set xb := x \in blacks _; set xg := x \in grays e.
@@ -354,7 +312,7 @@ Local Notation "x '<[' e ']=' y" := (precedes x y e)
 
 Record wf_num e := WfNum {
    wf_num0      : forall x, (num e x == 0) = (x \in whites e);
-   wf_num_infty : forall x, (num e x == infty) = (x \in cover (sccs e));
+   wf_num_infty : forall x, (num e x == infty) = (x \in cover (esccs e));
    wf_num_lt    : forall x, num e x != infty -> num e x < sn e;
    wf_sn        : sn e = #|grays e :|: blacks e|.+1;
    wf_num_stack : {in stack e &, forall x y,  (num e x <= num e y) = (y <[e]= x)}
@@ -371,7 +329,7 @@ Proof. by move=> e_n; rewrite inordK // ltnS leq_num_infty. Qed.
 
 Lemma num_inftyP e x : 
   wf_num e ->
-  reflect (num e x = infty) (x \in cover (sccs e)).
+  reflect (num e x = infty) (x \in cover (esccs e)).
 Proof. by case => _ <- _ _ _; apply/eqP. Qed.
 
 Lemma sn_small e : wf_num e -> sn e <= infty.
@@ -474,7 +432,7 @@ Record invariants (e : env) := Invariants {
   inv_wf_num   : wf_num e;
   inv_wf_graph : wf_graph e;
   wf_noblack_towhite : noblack_to_white e;
-  inv_sccs : sccs e = black_gsccs e;
+  inv_sccs : esccs e = black_gsccs e;
 }.
 
 Record pre_dfs (roots : {set V}) (e : env) := PreDfs {
@@ -539,7 +497,7 @@ Qed.
 Definition subenv e1 e2 :=
   [&&  grays e1 == grays e2,
        blacks e1 \subset blacks e2,
-       sccs e1 \subset sccs e2,
+       esccs e1 \subset esccs e2,
        [forall x in stack e1, num e2 x == num e1 x] &
        [exists n : 'I_infty, stack e1 == drop n (stack e2)]].
 
@@ -549,7 +507,7 @@ Proof. by move=> /and4P [/eqP]. Qed.
 Lemma subenv_blacks e1 e2 : subenv e1 e2 -> blacks e1 \subset blacks e2.
 Proof. by move=> /and4P []. Qed.
 
-Lemma subenv_sccs e1 e2 : subenv e1 e2 -> sccs e1 \subset sccs e2.
+Lemma subenv_sccs e1 e2 : subenv e1 e2 -> esccs e1 \subset esccs e2.
 Proof. by move=> /and4P []. Qed.
 
 Lemma subenv_num e1 e2 : subenv e1 e2 ->
@@ -770,7 +728,7 @@ split => //; first exact: subenv_trans sube2.
 rewrite m1_min m2_min split_wreach bigmin_setU /=.
 congr (minn (val _) _); apply: eq_bigr => y xy; apply/val_inj=> /=.
 rewrite !ord_num //.
-have /orP[ys|ysccs] : (y \in stack e1) || (y \in cover (sccs e1)).
+have /orP[ys|ysccs] : (y \in stack e1) || (y \in cover (esccs e1)).
 + suff: y \notin whites e1 by case: color4P.
   by rewrite whites1 inE xy.
 + exact/esym/subenv_num.
@@ -804,8 +762,8 @@ have xe_uniq : uniq (x :: stack e).
 have x_stack : x \in stack e1 by rewrite s_def mem_cat mem_head orbT.
 have x_grays : x \in grays e1.
    by rewrite (subenv_grays sube1) grays_add_stack ?setU11.
-have sx_subscc : is_subscc [set y in rcons s x].
-  apply: (@is_subscc1 x); first by rewrite inE mem_rcons mem_head.
+have sx_subscc : is_subscc edge [set y in rcons s x].
+  apply: (@is_subscc1 _ edge x); first by rewrite inE mem_rcons mem_head.
   move=> y; rewrite !inE mem_rcons in_cons => /predU1P [->//|y_s]; split.
     apply: (@wf_grays_to_stack e1) => //; first by rewrite s_def mem_cat y_s.
     rewrite wf_num_stack //s_def; last by rewrite mem_cat y_s.
@@ -903,7 +861,7 @@ case: ltnP => [m1_small|m1_big] //=.
       have /setU1P [eq_yx|//] := scc_sub y y_scc.
       rewrite eq_yx in y_scc.
       have x'_scc : (x' \in scc).
-        rewrite -(def_scc _ y_scc) // mem_scc /= x_to_x' /=.
+        rewrite -(def_scc scc_gsccs y_scc) // mem_scc /symconnect /= x_to_x' /=.
         by rewrite (wf_grays_to_stack e1_gwf) // ltnW.
       have /scc_sub := x'_scc.
       rewrite !inE (negPf neq_x'x) /=.
@@ -912,7 +870,7 @@ case: ltnP => [m1_small|m1_big] //=.
     + rewrite grays_add_blacks (subenv_grays sube1) grays_add_stack ?setU1K //.
       by rewrite whites_graysF.
     + by rewrite (subset_trans (subenv_blacks sube1)) // subsetUr.
-    + by rewrite -[sccs e]/(sccs (add_stack x e)) subenv_sccs.
+    + by rewrite -[esccs e]/(esccs (add_stack x e)) subenv_sccs.
     + apply/forall_inP => y y_stack; apply/eqP.
       rewrite (subenv_num sube1)/= ?in_cons ?y_stack ?orbT// ffunE/=.
       by rewrite ifN//; apply: contraTneq xe_uniq => <- /=; rewrite y_stack.
@@ -927,7 +885,7 @@ have numx_le y : y \in wreach e x -> num e1 y >= num e1 x.
   move=> xy; rewrite (@leq_trans m) //; last first.
     by rewrite sn_min -ord_num// geq_bigmin_cond.
   by rewrite (subenv_num sube1) ?mem_head//= ffunE/= eqxx. (*TODO: lemma*)
-have scc_max : scc_of x \subset [set y in s2].
+have scc_max : gscc_of x \subset [set y in s2].
   apply/subsetP=> y; rewrite inE=> y_sccx; apply: contraTT isT => yNs2.
   have xy : gconnect x y by have := y_sccx; rewrite mem_scc /= => /andP[].
   have x_s2 : x \in s2 by rewrite mem_rcons mem_head.
@@ -937,7 +895,7 @@ have scc_max : scc_of x \subset [set y in s2].
   move=> /connect1r [] // x' xx's2 /= /andP [x'_s2 x'y'] y'y.
   have xx' : gconnect x x'.
     by apply: connect_sub xx's2 => u v /= /andP[_]; apply: connect1.
-  have /or3P[] : [|| y' \in whites e1, y' \in cover (sccs e1)
+  have /or3P[] : [|| y' \in whites e1, y' \in cover (esccs e1)
                    | y' \in stack e1] by case: color4P.
   - move: x'_s2; rewrite mem_rcons in_cons => /predU1P [eq_x'x|x_s].
       by rewrite succ_whiteF -?eq_x'x.
@@ -945,9 +903,9 @@ have scc_max : scc_of x \subset [set y in s2].
     by move=> /pred0P /(_ y') /=; rewrite [_ \in _]x'y' /= => ->.
   - move=> /bigcupP [scc'].
     rewrite black_sccs1 inE => /andP[scc'_gsccs scc'_black].
-    move=> /def_scc - /(_ scc'_gsccs) eq_scc'; rewrite -eq_scc' in scc'_black.
-    have : x \in scc_of y'.
-      have:= y_sccx; rewrite !mem_scc /= andbC => /andP[yx _].
+    move=> /def_scc - /(_ _ scc'_gsccs) eq_scc'; rewrite -eq_scc' in scc'_black.
+    have : x \in gscc_of y'.
+      have:= y_sccx; rewrite !mem_scc /= /symconnect andbC => /andP[yx _].
       by rewrite (connect_trans y'y) //= (connect_trans xx') //= connect1.
     by move=> /(subsetP scc'_black); case: color4P x_grays.
   - rewrite s_def -cat_rcons mem_cat (negPf y'Ns2) /= => y'_stack.
@@ -958,7 +916,7 @@ have scc_max : scc_of x \subset [set y in s2].
       rewrite -(@uniq_catLR _ x' s2) ?mem_cat ?x'_s2 //.
       by rewrite cat_rcons -s_def wf_uniq.
     have s2_whites: {subset s2 <= whites e}.
-      move=> z z_s2; have: z \notin cover (sccs e).
+      move=> z z_s2; have: z \notin cover (esccs e).
         apply/negP=> /(subsetP (subset_cover (subenv_sccs sube1))).
         suff: z \in stack e1 by case: color4P.
         by rewrite s_def -cat_rcons mem_cat z_s2.
@@ -994,7 +952,7 @@ split=> //.
     * move=> y; rewrite !take_s.
       rewrite /cover big_setU1/= -/(cover _).
         by rewrite set_infty_eq_infty wf_num_infty// !inE.
-      suff: ~~ ([set y0 in rcons s x] \subset cover (sccs e1)).
+      suff: ~~ ([set y0 in rcons s x] \subset cover (esccs e1)).
         apply: contra => sx_in.
         by rewrite /cover (big_setD1 _ sx_in) /= subsetUl.
       apply: contraTN isT => /subsetP /(_ x); rewrite inE mem_rcons in_cons eqxx/=.
@@ -1056,12 +1014,12 @@ split=> //.
     have x_s2 : x \in [set y in s2] by rewrite inE mem_rcons mem_head.
     have s2_gsccs : [set y in rcons s x] \in gsccs.
       apply/imsetP => /=; exists x => //.
-      rewrite -[RHS](@def_scc _ x); last 2 first.
+      rewrite -[RHS](@def_scc _ edge _ x); last 2 first.
       * by apply/imsetP; exists x.
-      * by rewrite !inE ?connect0.
+      * by rewrite !inE /symconnect ?connect0.
       apply/eqP; rewrite eqEsubset scc_max.
       have [scc' scc'_gsccs sub'] := is_subscc_in_scc sx_subscc.
-      by rewrite (@def_scc scc') ?sub' //; apply: (subsetP sub').
+      by rewrite (@def_scc _ edge scc') ?sub' //; apply: (subsetP sub').
     have [scc_gsccs|] //= := boolP (scc \in gsccs); last first.
       by apply: contraNF; rewrite orbF => /eqP->.
     apply/idP/idP.
@@ -1070,7 +1028,7 @@ split=> //.
         by case: eqP=> [->|] //= _ => /(subsetP sb).
       by move=> /subset_trans; apply; rewrite subsetU1.
     have [x_scc|xNscc] := boolP (x \in scc).
-      by move=> _; rewrite -(def_scc _ x_scc) // (def_scc s2_gsccs) ?eqxx.
+      by move=> _; rewrite -(def_scc scc_gsccs x_scc) // (def_scc s2_gsccs) ?eqxx.
     rewrite -subDset (setDidPl _); first by move->; rewrite orbT.
     by rewrite disjoint_sym (@eq_disjoint1 _ x) // => y; rewrite !inE.
 - rewrite /= /subenv grays_add_sccs ?take_s ?sb ?g1Nx ?eqxx /= ?drop_s //=.
@@ -1154,7 +1112,7 @@ case: tarjan_rec => [m e] [].
   + by move=> x; rewrite ffunE.
   + by rewrite cards0.
   apply/setP=> y; rewrite !inE /= subset0 andbC; case: eqP => //= ->.
-  by have /and3P [_ _ /negPf->]:= gsccs_partition.
+  by have /and3P [_ _ /negPf->]:= sccs_partition edge.
 move=> [[stack_wf _ _ e_nwf] _ _] sccse /subenv_grays grayse.
 rewrite (eqP _ : \bigcup_(x in _) _ = setT) ?setDT => [whe ->|]; last first.
   rewrite -subTset; apply/subsetP=> y _; apply/bigcupP.
@@ -1163,20 +1121,20 @@ have blackse : blacks e = setT.
   move/eqP: whe; rewrite whitesE grayse grays0 set0U.
   by rewrite -subset0 subCset setC0 subTset => /eqP.
 rewrite /black_gsccs blackse ?grayse ?grays0 ?setTD ?set0U// in sccse stack_wf.
-have {sccse}sccse: sccs e = gsccs.
+have {sccse}sccse: esccs e = gsccs.
   by apply/setP=> scc; rewrite sccse inE subsetT andbT.
 have stacke : stack e = [::].
-  have := stack_wf; rewrite sccse cover_gsccs setCT.
+  have := stack_wf; rewrite sccse cover_sccs setCT.
   by case: stack => // x s /(_ x); rewrite !inE eqxx.
 have sne : sn e = infty.
   by rewrite wf_sn// grayse blackse grays0 set0U cardsT.
 have nume : num e = [ffun _ => infty].
   apply/ffunP => x; rewrite ffunE; apply/eqP; rewrite wf_num_infty//.
-  by rewrite sccse cover_gsccs.
+  by rewrite sccse cover_sccs.
 congr (_, _); last first.
   by case: (e) blackse sccse stacke sne nume => //= *; congr Env.
 rewrite big1 // => x _; apply/val_inj; rewrite /= ord_num//.
-by apply/eqP; rewrite wf_num_infty // sccse cover_gsccs.
+by apply/eqP; rewrite wf_num_infty // sccse cover_sccs.
 Qed.
 
 Theorem tarjan_correct : tarjan = gsccs.
